% recurrence-initial.tex

%%%%%%%%%%%%%%%
\begin{frame}{}
  \[
    T(n) = a T(n/b) + f(n)
  \]

  \fig{width = 0.75\textwidth}{figs/master-tree}

  \[
    T(n) = n^{\log_{b}{a}} \red{T(1)} + 
        \sum_{j = 0}^{\log_{b}{n} - 1} a^{j} f\left(\frac{n}{b^{j}}\right)
  \]
\end{frame}
%%%%%%%%%%%%%%%

%%%%%%%%%%%%%%%
\begin{frame}{}
  \[
    T(n) = a T(n/b) + f(n)
  \]
  \[
    T(n) = n^{\log_{b}{a}} \red{T(1)} + 
        \sum_{j = 0}^{\log_{b}{n} - 1} a^{j} f\left(\frac{n}{b^{j}}\right)
  \]

  \[
    \teal{\boxed{f(n) \;\text{\it vs.}\; n^{\log_{b}{a}}}}
  \]

  \begin{align*}
    f(n) = O(n^{\log_{b}{a} - \epsilon}) &\implies T(n) = \Theta(n^{\log_{b}{a}}) \\[8pt]
    \gray{f(n) = \Theta(n^{\log_{b}{a}})} &\gray{\implies T(n) = \Theta(n^{\log_{b}{a}} \log n)} \\[8pt]
    \gray{f(n) = \Omega(n^{\log_{b}{a} + \epsilon})} &\gray{\implies T(n) = \Theta(f(n))}
  \end{align*}
\end{frame}
%%%%%%%%%%%%%%%

%%%%%%%%%%%%%%%
\begin{frame}{}
  \[
    T(n) = n^{\log_{b}{a}} \red{T(1)} + 
        \sum_{j = 0}^{\log_{b}{n} - 1} a^{j} f\left( \frac{n}{b^{j}} \right)
  \]

  \pause
  \[
    \blue{a^{\log_{b}{n} - 1} f\left( \frac{n}{b^{\log_{b}{n} - 1}} \right) 
        = a^{\log_{b}{n} - 1} f(b) = a^{\log_{b}{n}} \frac{f(b)}{a}}
  \]

  \pause
  \begin{align*}
    T(n) &= n^{\log_{b}{a}} \red{T(1)} + 
        \sum_{j = 0}^{\log_{b}{n} - 1} a^{j} f\left(\frac{n}{b^{j}} \right) \\
        &= n^{\log_{b}{a}} \left( \purple{\frac{f(b^{\log_{b}{n}})}{a^{\log_{b}{n}}} + \ldots + \frac{f(b^2)}{a^2} + \frac{f(b)}{a}} + \red{T(1)} \right)
  \end{align*}

  \pause
  \begin{center}
    \purple{$f(n)$ is asymptotically positive.}
  \end{center}

  \pause
  \vspace{-0.30cm}
  \[
    \red{T(1) = d = \Theta(1), \quad (d \text{ can be } 0)}
  \]
\end{frame}
%%%%%%%%%%%%%%%

%%%%%%%%%%%%%%%
\begin{frame}{}
  \[
    T(n) = n^{\log_{b}{a}} \red{T(1)} + 
        \sum_{j = 0}^{\log_{b}{n} - 1} a^{j} f\left(\frac{n}{b^{j}}\right)
  \]

  \begin{align*}
    f(n) = O(n^{\log_{b}{a} - \epsilon}) &\implies T(n) = \Theta(n^{\log_{b}{a}}) 
    \\[6pt]
    \gray{f(n) = \Theta(n^{\log_{b}{a}})} &\gray{\implies T(n) = \Theta(n^{\log_{b}{a}} \log n)}
    \\[6pt]
    \gray{f(n) = \Omega(n^{\log_{b}{a} + \epsilon})} &\gray{\implies T(n) = \Theta(f(n))}
  \end{align*}

  \pause
  \[
    T(n) = n^{\log_{b}{a}} \left( \purple{\frac{f(b^{\log_{b}{n}})}{a^{\log_{b}{n}}} + \ldots 
        + \frac{f(b^2)}{a^2} + \frac{f(b)}{a}} + \red{T(1)} \right)
  \]

  \begin{center}
    \purple{$f(n)$ is asymptotically positive.}
  \end{center}

  \[
    \purple{\sum_{j = 0}^{\log_{b}{n} - 1} a^{j} f\left(\frac{n}{b^{j}}\right)} = \Omega(n^{\log_{b}{a}})
  \]
\end{frame}
%%%%%%%%%%%%%%%

%%%%%%%%%%%%%%%
\begin{frame}{}
  \[
    T(n) = a T(n/b) + f(n)
  \]

  \[
    T(n) = n^{\log_{b}{a}} \left( \purple{\frac{f(b^{\log_{b}{n}})}{a^{\log_{b}{n}}} + \ldots + \frac{f(b^2)}{a^2} + \frac{f(b)}{a}} + \red{T(1)} \right)
  \]

  \pause
  \vspace{0.30cm}
  \[
    \red{\text{What if } f(n) = 0?}
  \]

  \pause
  \[
    T(n) = n^{\log_{b}{a}} \red{T(1)}
  \]

  \pause
  \[
    T(n) = \begin{cases}
      0, & T(1) = 0 \\[5pt]
      \Theta(n^{\log_{b}{a}}), & T(1) = d \neq 0
    \end{cases}
  \]
\end{frame}
%%%%%%%%%%%%%%%

%%%%%%%%%%%%%%%
% \begin{frame}{}
%   \[
%     T(n) = T(\frac{n}{2}) + T(\frac{n}{4}) + T(\frac{n}{8}) + n \pause = \Theta(n)
%   \]
% \end{frame}
%%%%%%%%%%%%%%%

%%%%%%%%%%%%%%%
% \begin{frame}[fragile]{}
%   \[
%     T(n) = T(\frac{n}{2}) + T(\frac{n}{4}) + T(\frac{n}{8})
%   \]
% 
%   \pause
%   \[
%     T(n) = \begin{cases}
%       0, & T(1) = 0 \\[5pt]
%       \teal{\Theta(n^{0.879146})}, & T(1) = d \neq 0
%     \end{cases}
%   \]
% 
%   \pause
%   \vspace{0.30cm}
%   \[
%     \boxed{\red{T(n) = \Theta(n^\alpha)}}
%   \]
% 
%   \pause
%   \vspace{0.30cm}
%   \[
%     2^{-\alpha} + 4^{-\alpha} + 8^{-\alpha} = 1
%   \]
% 
%   \pause
%   \vspace{0.30cm}
%   \begin{center}
%     \begin{verbatim}
%       Solve[2^{-x} + 4^{-x} + 8^{-x} == 1, x] // N
%     \end{verbatim}
%   \end{center}
% \end{frame}
%%%%%%%%%%%%%%%