%%%%%%%%%%%%%%%
\begin{frame}{}
  \[
    f: A \to B,\; A_0 \subseteq A,\; B_0 \subseteq B
  \]

  \begin{definition}[Image]
    The \blue{image} of $A_0$ under $f$ is the set

    \[
      f(A_0) = \set{f(a) \mid a \in A_0}.
    \]
  \end{definition}

  \vspace{0.60cm}
  \begin{definition}[Inverse Image]
    The \blue{inverse image} of $B_0$ under $f$ is the set
    \[
      f^{-1}(B_0) = \set{a \in A \mid f(a) \in B_0}.
    \]
  \end{definition}
\end{frame}
%%%%%%%%%%%%%%%

%%%%%%%%%%%%%%%
\begin{frame}{}
  \begin{theorem}[Properties of $f$ and $f^{-1}$ (Theorem $16.7$)]
    \[
      f: A \to B,\; A_0, A_1, A_2 \subseteq A,\; B_0, B_1, B_2 \subseteq B
    \]

    \vspace{-0.10cm}
    \begin{enumerate}[(i)]
      \setlength{\itemsep}{8pt}
      \item $f$, when applied to subsets of $A$, preserves only ``$\subseteq$'' and $\cup$:
	\begin{enumerate}[(1)]
	  \setlength{\itemsep}{4pt}
	  \item $A_1 \subseteq A_2 \implies f(A_1) \subseteq f(A_2)$
	  \item $f(A_1 \cup A_2) = f(A_1) \cup f(A_2)$
	  \item $f(A_1 \cap A_2) \red{\;\subseteq\;} f(A_1) \cap f(A_2)$
	  \item $f(A \setminus A_0) \neq B \setminus f(A_0)$
	\end{enumerate}
      \item $f^{-1}$, when applied to subsets of $B$, preserves $\subseteq, \cup, \cap,$ and $\setminus$:
	\begin{enumerate}[(1)]
	  \setlength{\itemsep}{4pt}
	  \setcounter{enumii}{4}
	  \item $B_1 \subseteq B_2 \implies f^{-1}(B_1) \subseteq f^{-1}(B_2)$
	  \item $f^{-1}(B_1 \cup B_2) = f^{-1}(B_1) \cup f^{-1}(B_2)$
	  \item $f^{-1}(B_1 \cap B_2) \red{\;=\;} f^{-1}(B_1) \cap f^{-1}(B_2)$
	  \item $f^{-1}(B \setminus B_0) = A \setminus f^{-1}(B_0)$
	\end{enumerate}
    \end{enumerate}
  \end{theorem}
\end{frame}
%%%%%%%%%%%%%%%

%%%%%%%%%%%%%%%
\begin{frame}{}
  \begin{theorem}[Properties of $f$ and $f^{-1}$ (Theorem $16.7$)]
    \[
      f: A \to B,\; A_0 \subseteq A,\; B_0 \subseteq B
    \]

    \vspace{-0.10cm}
    \begin{enumerate}[(i)]
      \setcounter{enumi}{2}
      \item $f$ and $f^{-1}$: \\[8pt]
	\begin{enumerate}[(1)]
	  \setlength{\itemsep}{15pt}
	  \setcounter{enumii}{8}
	    \item $A_0 \subseteq f^{-1}(f(A_0))$
	      \centerline{\red{$Q$:} When is $A_0 = f^{-1}(f(A_0))?$}
	    \pause
	    \item $B_0 \subseteq f(f^{-1}(B_0))$
	      \centerline{\red{$Q$:} When is $B_0 = f(f^{-1}(B_0))?$}
	\end{enumerate}
    \end{enumerate}
  \end{theorem}
\end{frame}
%%%%%%%%%%%%%%%

%%%%%%%%%%%%%%%
\begin{frame}{}
  \begin{exampleblock}{Problem $16.20$}
    \[
      f: A \to B, \quad A_1, A_2 \subseteq A
    \]

    \begin{enumerate}[(i)]
      \centering
      \item When is $f(A_1) = f(A_2) \implies A_1 = A_2?$
    \end{enumerate}
  \end{exampleblock}
\end{frame}
%%%%%%%%%%%%%%%

%%%%%%%%%%%%%%%
\begin{frame}{}
  \begin{exampleblock}{Problem $16.21$}
    \[
      f: A \to B, \quad B_1, B_2 \subseteq B
    \]

    \begin{enumerate}[(i)]
      \centering
      \item When is $f^{-1}(B_1) = f^{-1}(B_2) \implies B_1 = B_2?$
    \end{enumerate}
  \end{exampleblock}
\end{frame}
%%%%%%%%%%%%%%%
