% file: parts/searching-analysis.tex

%%%%%%%%%%%%%%%
\begin{frame}{}
  \begin{exampleblock}{Searching an Unsorted Array (CLRS Problem $5-2\; (f)$)}
    \input{algs/deterministic-search}

    \pause
    \begin{enumerate}[(a)]
      \setcounter{enumi}{4}
      \item \[ \exists!\; i: A[i] = x \]
      \item \[ \exists!_{k}\; i: A[i] = x \]
    \end{enumerate}
  \end{exampleblock}
\end{frame}
%%%%%%%%%%%%%%%

%%%%%%%%%%%%%%%
\begin{frame}{}
  \[ 
    \exists!\; i: A[i] = x 
  \]

  \pause
  \[
    \red{Y: \# \text{ of comparisons}}
  \]

  \pause
  \begin{align*}
    \E[Y] &= \sum_{y = 1}^{n} y \Pr\set{Y = y} \\
    \onslide<4->{&= \sum_{y = 1}^{n} y \Pr\set{A[y] = x} \\}
    \onslide<5->{&= \frac{1}{n} \sum_{y = 1}^{n} y \\}
    \onslide<6->{&= \frac{n+1}{2}}
  \end{align*}
\end{frame}
%%%%%%%%%%%%%%%

%%%%%%%%%%%%%%%
\begin{frame}{}
  \[ 
    \exists!_{k}\; i: A[i] = x 
  \]

  \pause
  \[
    \red{Y: \# \text{ of comparisons}}
  \]

  \pause
  \vspace{-0.50cm}
  \begin{align*}
    \E[Y] &= \sum_{y = 1}^{\red{n-k+1}} y \Pr\set{Y = y} \\
    \onslide<4->{&= \sum_{y = 1}^{n-k+1} y \Pr\set{y \text{ is the first index among $k$ indices {\it s.t.} } A[y] = x} \\}
    \onslide<5->{&= \sum_{y = 1}^{n-k+1} y \red{\frac{\binom{n-y}{k-1}}{\binom{n}{k}}}}
    \onslide<6->{= \frac{1}{\binom{n}{k}} \teal{\sum_{y = 1}^{n-k+1} y \binom{n-y}{k-1}} \\}
    \onslide<7->{&= \frac{1}{\binom{n}{k}} \purple{\binom{n+1}{k+1}} = \frac{n+1}{k+1}}
  \end{align*}

  \uncover<8->{
    \[
      k = 1 \implies \E[Y] = \frac{n+1}{2}, \qquad k = n \implies \E[Y] = 1
    \]
  }
\end{frame}
%%%%%%%%%%%%%%%

%%%%%%%%%%%%%%%
\begin{frame}{}
  \begin{exampleblock}{After-class Exercise}
    \[
      \sum_{y=1}^{n-k+1} y \binom{n-y}{k-1} = \binom{n+1}{k+1}
    \]
  \end{exampleblock}

  \begin{columns}
    \column{0.50\textwidth}
      \fignocaption{width = 0.45\textwidth}{figs/concrete-mathematics}{\centerline{\small Chapter $5$: Binomial Coefficients}}
    \column{0.50\textwidth}
      \[
	r \binom{r-1}{k-1} = k \binom{r}{k}
      \]

      \vspace{0.60cm}
      \[
	\sum_{0 \le k \le n} \binom{k}{m} = \binom{n+1}{m+1}
      \]
  \end{columns}
\end{frame}
%%%%%%%%%%%%%%%

%%%%%%%%%%%%%%%
\begin{frame}{}
  \begin{align*}
    \sum_{y=1}^{n-k+1} y \binom{n-y}{k-1} &= \sum_{y=0}^{n-k} (y+1) \binom{n-y-1}{k-1} \\
    &= \sum_{y=0}^{n-k} \big((n+1) - (n-y)\big) \binom{n-y-1}{k-1} \\
    &= \sum_{y=0}^{n-k} (n+1) \binom{n-y-1}{k-1} - \sum_{y=0}^{n-k} (n-y) \binom{n-y-1}{k-1} \\
    &= (n+1) \sum_{y=0}^{n-k}\binom{n-y-1}{k-1} - k \sum_{y=0}^{n-k} \binom{n-y}{k} \\
    &= (n+1) \sum_{m=k-1}^{n-1}\binom{m}{k-1} - k \sum_{m=k}^{n} \binom{m}{k} \\
    &= (n+1) \binom{n}{k} - k \binom{n+1}{k+1} = \binom{n+1}{k+1}
  \end{align*}
\end{frame}
%%%%%%%%%%%%%%%

%%%%%%%%%%%%%%%
\begin{frame}{}
  \centerline{\teal{\large Indicator Random Variables}}
\end{frame}
%%%%%%%%%%%%%%%

%%%%%%%%%%%%%%%
\begin{frame}{}
\end{frame}
%%%%%%%%%%%%%%%
