% file: 9-equal.tex

%%%%%%%%%%%%%%%
\begin{frame}{}
  \begin{exampleblock}{$\texttt{equal}(S_1,S_2)$ (Problem $5.9$)}
    \begin{itemize}
      \item $\texttt{head}(X)$
      \item $\texttt{tail}(X)$
      \item $\texttt{last}(X)$
      \item $\texttt{all-but-last}(X)$
      \item $\texttt{eq}(s,t)$
    \end{itemize}
  \end{exampleblock}
\end{frame}
%%%%%%%%%%%%%%%

%%%%%%%%%%%%%%%
\begin{frame}[fragile]{}
  \begin{columns}
    \column{0.50\textwidth}
  \begin{lstlisting}[style = CStyle]
 while $X \neq \Lambda \land Y \neq \Lambda$
   if $\texttt{eq}(\texttt{head}(X), \texttt{head}(Y))$
     $X \gets \texttt{tail}(X)$
     $Y \gets \texttt{tail}(Y)$
   else
     return false

 if $X = \Lambda \land Y = \Lambda$
   return true
 return false
  \end{lstlisting}
    \column{0.50\textwidth}
  \begin{lstlisting}[style = CStyle]
 $X \gets S_1$
 $Y \gets S_2$

 $E \gets \top$
 |\uncover<3->{\cyan{//} \red{$S_1 = S_2 \iff E = \top \land X = Y$}}|
 while $X \neq \Lambda \land Y \neq \Lambda \land E = \top$
   if $\texttt{eq}(\texttt{head}(X), \texttt{head}(Y))$
     $X \gets \texttt{tail}(X)$
     $Y \gets \texttt{tail}(Y)$
   else
     $E \gets \bot$

 if $\lnot (X = \Lambda \land Y = \Lambda)$
   $E \gets \bot$
 |\uncover<2->{\cyan{//} \red{$S_1 = S_2 \iff E = \top$}}|

 return $E$
  \end{lstlisting}
  \end{columns}

% |\uncover<2->{$X \gets S_1$}|
% |\uncover<2->{$Y \gets S_2$}|
% // |\red{$I:$} \teal{$S_1 = S_2 \iff X = Y$}|
% // |\teal{$S_1 = S_2 \iff X = Y \land \lnot(X \neq \Lambda \land Y \neq \Lambda)$}|
\end{frame}
%%%%%%%%%%%%%%%

%%%%%%%%%%%%%%%
\begin{frame}[fragile]{}
  \begin{lstlisting}[style = CStyle]
  肖江
  \end{lstlisting}
\end{frame}
%%%%%%%%%%%%%%%

%%%%%%%%%%%%%%%
\begin{frame}[fragile]{}
  \begin{lstlisting}[style = CStyle]
    $X \gets S_1$
    $Y \gets S_2$

    $E \gets \top$
    while $X \neq \Lambda \land E == \top$
      if $Y == \Lambda$
        $E \gets \bot$
      else if $\texttt{eq}(\texttt{head}(X), \texttt{head}(Y))$
          $X \gets \texttt{tail}(X)$
          $Y \gets \texttt{tail}(Y)$
      else
        $E \gets \bot$

    if $Y \neq \Lambda$
      $E \gets \bot$

    return $E$
  \end{lstlisting}
\end{frame}
%%%%%%%%%%%%%%%
